src/riscv/Platform/MetricMinimal.v
@@ -64,12 +64,12 @@ Section Riscv.
     fence := liftL2 id fence;
     endCycleNormal := liftL0 (addMetricInstructions 1) endCycleNormal;
     endCycleEarly{A} := liftL0 (addMetricInstructions 1) (@endCycleEarly _ _ _ _ _ A);
-    }.
+  }.
 
-  Instance IsMetricRiscvMachineWithLeakage: @RiscvProgramWithLeakage width BW word (OState MetricRiscvMachine) _ _ _ := {
+  Instance IsMetricRiscvMachineWithLeakage: @RiscvProgramWithLeakage _ _ _ (OState MetricRiscvMachine) _ _ _ := {
       RVP := IsMetricRiscvMachine;
       leakEvent := liftL1 id leakEvent;
-      }.
+  }.
 
   Arguments Memory.load_bytes: simpl never.
   Arguments Memory.store_bytes: simpl never.
